Modify the extraction to use pbytes for memory representation, optimise packed and unpacked load/store operations.

WebAssembly/Wasm_Memory_Printing.thy
@@ -1,4 +1,224 @@
-theory Wasm_Memory_Printing imports Wasm_Base_Defs Wasm_Type_Printing begin
+theory Wasm_Memory_Printing imports Wasm_Base_Defs Wasm_Type_Printing Wasm_Interpreter begin
+
+
+definition mem_rep_read_i32 :: "mem_rep \<Rightarrow> nat \<Rightarrow> i32" where
+  "mem_rep_read_i32 m n = deserialise_i32 (mem_rep_read_bytes m n (t_num_length T_i32))"
+
+definition mem_rep_read_i64 :: "mem_rep \<Rightarrow> nat \<Rightarrow> i64" where
+  "mem_rep_read_i64 m n = deserialise_i64 (mem_rep_read_bytes m n (t_num_length T_i64))"
+
+definition mem_rep_read_f32 :: "mem_rep \<Rightarrow> nat \<Rightarrow> f32" where
+  "mem_rep_read_f32 m n = deserialise_f32 (mem_rep_read_bytes m n (t_num_length T_f32))"
+
+definition mem_rep_read_f64 :: "mem_rep \<Rightarrow> nat \<Rightarrow> f64" where
+  "mem_rep_read_f64 m n = deserialise_f64 (mem_rep_read_bytes m n (t_num_length T_f64))"
+
+definition load_v_num' :: "mem \<Rightarrow> nat \<Rightarrow> off \<Rightarrow> t_num \<Rightarrow> v_num option" where
+  "load_v_num' m n off t = 
+  (let l = t_num_length t in
+  (if (mem_length m \<ge> (n+off+l)) then
+    (case t of
+      T_i32 \<Rightarrow> Some (ConstInt32 (mem_rep_read_i32 (snd m) (n+off)))
+    | T_i64 \<Rightarrow> Some (ConstInt64 (mem_rep_read_i64 (snd m) (n+off)))
+    | T_f32 \<Rightarrow> Some (ConstFloat32 (mem_rep_read_f32 (snd m) (n+off)))
+    | T_f64 \<Rightarrow> Some (ConstFloat64 (mem_rep_read_f64 (snd m) (n+off)))
+  ) else None))"
+
+definition mem_rep_read_i32_of_i8 :: "mem_rep \<Rightarrow> nat \<Rightarrow> i32" where
+  "mem_rep_read_i32_of_i8 m n =  deserialise_i32 ((sign_extend S (t_num_length T_i32)) (mem_rep_read_bytes m n (tp_num_length Tp_i8)))"
+
+definition mem_rep_read_i32_of_u8 :: "mem_rep \<Rightarrow> nat \<Rightarrow> i32" where
+  "mem_rep_read_i32_of_u8 m n =  deserialise_i32 ((sign_extend U (t_num_length T_i32)) (mem_rep_read_bytes m n (tp_num_length Tp_i8)))"
+
+definition mem_rep_read_i32_of_i16 :: "mem_rep \<Rightarrow> nat \<Rightarrow> i32" where
+  "mem_rep_read_i32_of_i16 m n =  deserialise_i32 ((sign_extend S (t_num_length T_i32)) (mem_rep_read_bytes m n (tp_num_length Tp_i16)))"
+
+definition mem_rep_read_i32_of_u16 :: "mem_rep \<Rightarrow> nat \<Rightarrow> i32" where
+  "mem_rep_read_i32_of_u16 m n =  deserialise_i32 ((sign_extend U (t_num_length T_i32)) (mem_rep_read_bytes m n (tp_num_length Tp_i16)))"
+
+definition mem_rep_read_i32_of_i32 :: "mem_rep \<Rightarrow> nat \<Rightarrow> i32" where
+  "mem_rep_read_i32_of_i32 =  mem_rep_read_i32"
+
+definition mem_rep_read_i32_of_u32 :: "mem_rep \<Rightarrow> nat \<Rightarrow> i32" where
+  "mem_rep_read_i32_of_u32 =  mem_rep_read_i32"
+
+definition mem_rep_read_i64_of_i8 :: "mem_rep \<Rightarrow> nat \<Rightarrow> i64" where
+  "mem_rep_read_i64_of_i8 m n =  deserialise_i64 ((sign_extend S (t_num_length T_i64)) (mem_rep_read_bytes m n (tp_num_length Tp_i8)))"
+
+definition mem_rep_read_i64_of_u8 :: "mem_rep \<Rightarrow> nat \<Rightarrow> i64" where
+  "mem_rep_read_i64_of_u8 m n =  deserialise_i64 ((sign_extend U (t_num_length T_i64)) (mem_rep_read_bytes m n (tp_num_length Tp_i8)))"
+
+definition mem_rep_read_i64_of_i16 :: "mem_rep \<Rightarrow> nat \<Rightarrow> i64" where
+  "mem_rep_read_i64_of_i16 m n =  deserialise_i64 ((sign_extend S (t_num_length T_i64)) (mem_rep_read_bytes m n (tp_num_length Tp_i16)))"
+
+definition mem_rep_read_i64_of_u16 :: "mem_rep \<Rightarrow> nat \<Rightarrow> i64" where
+  "mem_rep_read_i64_of_u16 m n =  deserialise_i64 ((sign_extend U (t_num_length T_i64)) (mem_rep_read_bytes m n (tp_num_length Tp_i16)))"
+
+definition mem_rep_read_i64_of_i32 :: "mem_rep \<Rightarrow> nat \<Rightarrow> i64" where
+  "mem_rep_read_i64_of_i32 m n =  deserialise_i64 ((sign_extend S (t_num_length T_i64)) (mem_rep_read_bytes m n (tp_num_length Tp_i32)))"
+
+definition mem_rep_read_i64_of_u32 :: "mem_rep \<Rightarrow> nat \<Rightarrow> i64" where
+  "mem_rep_read_i64_of_u32 m n=  deserialise_i64 ((sign_extend U (t_num_length T_i64)) (mem_rep_read_bytes m n (tp_num_length Tp_i32)))"
+
+definition mem_rep_read_i64_of_i64 :: "mem_rep \<Rightarrow> nat \<Rightarrow> i64" where
+  "mem_rep_read_i64_of_i64 =  mem_rep_read_i64"
+
+definition mem_rep_read_i64_of_u64 :: "mem_rep \<Rightarrow> nat \<Rightarrow> i64" where
+  "mem_rep_read_i64_of_u64 =  mem_rep_read_i64"
+
+definition mem_rep_read_i32_packed :: "mem_rep \<Rightarrow> nat \<Rightarrow> sx \<Rightarrow> tp_num \<Rightarrow> i32" where
+  "mem_rep_read_i32_packed m n sx tp = (case (sx, tp) of
+    (S,Tp_i8) \<Rightarrow> mem_rep_read_i32_of_i8 m n
+  | (U,Tp_i8) \<Rightarrow> mem_rep_read_i32_of_u8 m n
+  | (S,Tp_i16) \<Rightarrow> mem_rep_read_i32_of_i16 m n
+  | (U,Tp_i16) \<Rightarrow> mem_rep_read_i32_of_u16 m n
+  | (S,Tp_i32) \<Rightarrow> mem_rep_read_i32_of_i32 m n
+  | (U,Tp_i32) \<Rightarrow> mem_rep_read_i32_of_u32 m n)"
+
+definition mem_rep_read_i64_packed :: "mem_rep \<Rightarrow> nat \<Rightarrow> sx \<Rightarrow> tp_num \<Rightarrow> i64" where
+  "mem_rep_read_i64_packed m n sx tp = (case (sx, tp) of
+    (S,Tp_i8) \<Rightarrow> mem_rep_read_i64_of_i8 m n
+  | (U,Tp_i8) \<Rightarrow> mem_rep_read_i64_of_u8 m n
+  | (S,Tp_i16) \<Rightarrow> mem_rep_read_i64_of_i16 m n
+  | (U,Tp_i16) \<Rightarrow> mem_rep_read_i64_of_u16 m n
+  | (S,Tp_i32) \<Rightarrow> mem_rep_read_i64_of_i32 m n
+  | (U,Tp_i32) \<Rightarrow> mem_rep_read_i64_of_u32 m n)"
+
+definition load_packed_v_num' :: "sx \<Rightarrow> mem \<Rightarrow> nat \<Rightarrow> off \<Rightarrow> t_num \<Rightarrow> tp_num \<Rightarrow> v_num option" where
+  "load_packed_v_num' sx m n off t tp = (
+    (if (mem_length m) \<ge> (n+off+(tp_num_length tp)) then
+      (case t of
+        T_i32 \<Rightarrow> Some (ConstInt32 (mem_rep_read_i32_packed (snd m) (n+off) sx tp))
+      | T_i64 \<Rightarrow> Some (ConstInt64 (mem_rep_read_i64_packed (snd m) (n+off) sx tp))
+      | T_f32 \<Rightarrow> Some (ConstFloat32 (deserialise_f32 ((sign_extend sx (t_num_length T_i32)) (mem_rep_read_bytes (snd m) (n+off) (tp_num_length tp))) ))
+      | T_f64 \<Rightarrow> Some (ConstFloat64 (deserialise_f64 ((sign_extend sx (t_num_length T_i64)) (mem_rep_read_bytes (snd m) (n+off) (tp_num_length tp))) ))
+    )
+   else None))"
+
+lemma load_packed_v_num_is[code]: "load_packed_v_num sx m n off t tp = load_packed_v_num' sx m n off t tp"
+proof -
+  have 1: "\<And> n m k sx. n+k \<le> mem_rep_length m \<Longrightarrow> (mem_rep_read_bytes m n k) = (sign_extend sx k (mem_rep_read_bytes m n k))"
+    unfolding mem_rep_read_bytes_def  unfolding mem_rep_length_def
+    sign_extend_def bytes_takefill_def by (auto simp add: takefill_same')
+  show ?thesis
+  apply (cases "load m n off (tp_num_length tp)")
+  unfolding mem_rep_read_i32_packed_def mem_rep_read_i64_packed_def load_packed_v_num_def load_packed_v_num'_def
+    mem_rep_read_i32_of_i8_def
+    mem_rep_read_i32_of_u8_def
+    mem_rep_read_i32_of_i16_def
+    mem_rep_read_i32_of_u16_def
+    mem_rep_read_i32_of_i32_def
+    mem_rep_read_i32_of_u32_def
+    mem_rep_read_i64_of_i8_def
+    mem_rep_read_i64_of_u8_def
+    mem_rep_read_i64_of_i16_def
+    mem_rep_read_i64_of_u16_def
+    mem_rep_read_i64_of_i32_def
+    mem_rep_read_i64_of_u32_def
+    mem_rep_read_i32_def
+    using t_num_length_def tp_num_length_def
+    apply (auto simp add: read_bytes_def wasm_deserialise_num_def load_def split: if_splits t_num.splits tp_num.splits sx.splits option.splits)
+    using mem_length_def 1[of "n+off" "4" "snd m"] 1[of "n+off" "8" "snd m"]
+    by auto  
+qed
+
+lemma load_v_num_is[code]: "load_v_num m n off t = load_v_num' m n off t"
+  unfolding load_v_num_def load_v_num'_def load_def
+            write_bytes_def
+            mem_rep_read_i32_def 
+            mem_rep_read_i64_def
+            mem_rep_read_f32_def 
+            mem_rep_read_f64_def
+            wasm_deserialise_num_def
+            read_bytes_def
+            mem_rep_read_bytes_def
+  by (auto split: t_num.splits v_num.splits)
+
+definition mem_rep_write_i32 :: "mem_rep \<Rightarrow> nat \<Rightarrow> i32 \<Rightarrow> mem_rep" where
+  "mem_rep_write_i32 m n val = mem_rep_write_bytes m n (serialise_i32 val)"
+
+definition mem_rep_write_i64 :: "mem_rep \<Rightarrow> nat \<Rightarrow> i64 \<Rightarrow> mem_rep" where
+  "mem_rep_write_i64 m n val = mem_rep_write_bytes m n (serialise_i64 val)"
+
+definition mem_rep_write_f32 :: "mem_rep \<Rightarrow> nat \<Rightarrow> f32 \<Rightarrow> mem_rep" where
+  "mem_rep_write_f32 m n val = (mem_rep_write_bytes m n (serialise_f32 val))"
+
+definition mem_rep_write_f64 :: "mem_rep \<Rightarrow> nat \<Rightarrow> f64 \<Rightarrow> mem_rep" where
+  "mem_rep_write_f64 m n val = mem_rep_write_bytes m n (serialise_f64 val)"
+
+
+definition mem_rep_write_i8_of_i32 :: "mem_rep \<Rightarrow> nat \<Rightarrow> i32 \<Rightarrow> mem_rep" where
+  "mem_rep_write_i8_of_i32 m n val = mem_rep_write_bytes m n (bytes_takefill zero_byte (tp_num_length Tp_i8) (serialise_i32 val))"
+
+definition mem_rep_write_i16_of_i32 :: "mem_rep \<Rightarrow> nat \<Rightarrow> i32 \<Rightarrow> mem_rep" where
+  "mem_rep_write_i16_of_i32 m n val = mem_rep_write_bytes m n (bytes_takefill zero_byte (tp_num_length Tp_i16) (serialise_i32 val))"
+
+definition mem_rep_write_i32_of_i32 :: "mem_rep \<Rightarrow> nat \<Rightarrow> i32 \<Rightarrow> mem_rep" where
+  "mem_rep_write_i32_of_i32 m n val = mem_rep_write_bytes m n (bytes_takefill zero_byte (tp_num_length Tp_i32) (serialise_i32 val))"
+
+definition mem_rep_write_i8_of_i64 :: "mem_rep \<Rightarrow> nat \<Rightarrow> i64 \<Rightarrow> mem_rep" where
+  "mem_rep_write_i8_of_i64 m n val = mem_rep_write_bytes m n (bytes_takefill zero_byte (tp_num_length Tp_i8) (serialise_i64 val))"
+
+definition mem_rep_write_i16_of_i64 :: "mem_rep \<Rightarrow> nat \<Rightarrow> i64 \<Rightarrow> mem_rep" where
+  "mem_rep_write_i16_of_i64 m n val = mem_rep_write_bytes m n (bytes_takefill zero_byte (tp_num_length Tp_i16) (serialise_i64 val))"
+
+definition mem_rep_write_i32_of_i64 :: "mem_rep \<Rightarrow> nat \<Rightarrow> i64 \<Rightarrow> mem_rep" where
+  "mem_rep_write_i32_of_i64 m n val = mem_rep_write_bytes m n (bytes_takefill zero_byte (tp_num_length Tp_i32) (serialise_i64 val))"
+
+definition store_packed_v_num' :: "mem \<Rightarrow> nat \<Rightarrow> off \<Rightarrow> v_num \<Rightarrow> tp_num \<Rightarrow> mem option" where
+  "store_packed_v_num' m n off v tp =
+    (if mem_length m \<ge> n + off + (tp_num_length tp) then 
+      Some (fst m, (case v of
+        ConstInt32 val \<Rightarrow>
+          (case tp of
+            Tp_i8 \<Rightarrow> mem_rep_write_i8_of_i32 (snd m) (n+off) val
+          | Tp_i16 \<Rightarrow> mem_rep_write_i16_of_i32 (snd m) (n+off) val
+          | Tp_i32 \<Rightarrow> mem_rep_write_i32_of_i32 (snd m) (n+off) val)
+      | ConstInt64 val \<Rightarrow>
+          (case tp of
+            Tp_i8 \<Rightarrow> mem_rep_write_i8_of_i64 (snd m) (n+off) val
+          | Tp_i16 \<Rightarrow> mem_rep_write_i16_of_i64 (snd m) (n+off) val
+          | Tp_i32 \<Rightarrow> mem_rep_write_i32_of_i64 (snd m) (n+off) val)
+      | ConstFloat32 val \<Rightarrow> mem_rep_write_bytes (snd m) (n + off)
+           (bytes_takefill zero_byte (tp_num_length tp) (serialise_f32 val))
+      | ConstFloat64 val \<Rightarrow> mem_rep_write_bytes (snd m) (n + off)
+           (bytes_takefill zero_byte (tp_num_length tp) (serialise_f64 val))))
+   else None)"
+
+lemma store_packed_v_num_is[code]: "store_packed_v_num m n off v tp = store_packed_v_num' m n off v tp"
+  unfolding store_packed_v_num_def store_packed_v_num'_def store_def write_bytes_def
+  mem_rep_write_i8_of_i32_def
+  mem_rep_write_i16_of_i32_def
+  mem_rep_write_i32_of_i32_def
+  mem_rep_write_i8_of_i64_def
+  mem_rep_write_i16_of_i64_def
+  mem_rep_write_i32_of_i64_def
+  bits_num_def
+  by (auto split: if_splits tp_num.splits v_num.splits)
+
+definition store_v_num' :: "mem \<Rightarrow> nat \<Rightarrow> off \<Rightarrow> v_num \<Rightarrow> mem option" where
+  "store_v_num' m n off vn = (let l = (t_num_length (typeof_num vn)) in
+    (if (mem_length m \<ge> (n+off+l)) then
+      (case vn of 
+        ConstInt32 val \<Rightarrow> Some (fst m, mem_rep_write_i32 (snd m) (n+off) val)
+      | ConstInt64 val \<Rightarrow> Some (fst m, mem_rep_write_i64 (snd m) (n+off) val)
+      | ConstFloat32 val \<Rightarrow> Some (fst m, mem_rep_write_f32 (snd m) (n+off) val)
+      | ConstFloat64 val \<Rightarrow> Some (fst m, mem_rep_write_f64 (snd m) (n+off) val))
+    else None))"
+
+lemma store_v_num_is[code]: "store_v_num m n off v = store_v_num' m n off v"
+  unfolding store_v_num_def store_v_num'_def store_def
+            write_bytes_def
+            mem_rep_write_i32_def 
+            mem_rep_write_i64_def
+            mem_rep_write_f32_def 
+            mem_rep_write_f64_def
+  apply (auto split: v_num.splits)
+  unfolding word_rsplit_rev_def bits_num_def bytes_takefill_def
+            serialise_i32_def
+            serialise_i64_def
+  using typeof_num_def t_num_length_def takefill_same serialise_f32_len serialise_f64_len
+  by (auto simp add: takefill_same' split: t_num.splits)
 
 (* Perhaps a more appropriate place for ocaml_int and related conversions is in Wasm_Type_Printing *)
 (* But right now it is only used for Parray memory representation *)
@@ -7,11 +227,15 @@ typedecl ocaml_int
 consts
   ocaml_int_to_integer :: "ocaml_int \<Rightarrow> integer"
   integer_to_ocaml_int :: "integer \<Rightarrow> ocaml_int"
+  ocaml_int_to_ocaml_i32_s :: "ocaml_int \<Rightarrow> ocaml_i32"
+  ocaml_int_to_ocaml_i64_s :: "ocaml_int \<Rightarrow> ocaml_i64"
 
 code_printing
   type_constructor ocaml_int \<rightharpoonup> (OCaml) "Int.t"
 | constant ocaml_int_to_integer \<rightharpoonup> (OCaml) "Z.of'_int"
 | constant integer_to_ocaml_int \<rightharpoonup> (OCaml) "Z.to'_int"
+| constant ocaml_int_to_ocaml_i32_s \<rightharpoonup> (OCaml) "I32Wrapper'_convert.of'_int'_s"
+| constant ocaml_int_to_ocaml_i64_s \<rightharpoonup> (OCaml) "I64Wrapper'_convert.of'_int'_s"
 
 definition ocaml_int_to_nat :: "ocaml_int \<Rightarrow> nat" where
   "ocaml_int_to_nat x = nat_of_integer (ocaml_int_to_integer x)"
@@ -20,28 +244,75 @@ definition nat_to_ocaml_int :: "nat \<Rightarrow> ocaml_int" where
   "nat_to_ocaml_int x = integer_to_ocaml_int (integer_of_nat x)"
 
 consts
-  ocaml_mem_rep_length :: "mem_rep \<Rightarrow> ocaml_int"
-  ocaml_mem_rep_mk :: "ocaml_int \<Rightarrow> byte \<Rightarrow> mem_rep"
-  ocaml_mem_rep_byte_at :: "mem_rep \<Rightarrow> ocaml_int \<Rightarrow> byte"
-  ocaml_mem_rep_read_bytes :: "mem_rep \<Rightarrow> ocaml_int \<Rightarrow> ocaml_int \<Rightarrow> bytes"
-  ocaml_mem_rep_write_bytes :: "mem_rep \<Rightarrow> ocaml_int \<Rightarrow> bytes \<Rightarrow> mem_rep"
-  ocaml_mem_rep_append :: "mem_rep \<Rightarrow> ocaml_int \<Rightarrow> byte \<Rightarrow> mem_rep"
+  ocaml_mem_rep_pbytes_length :: "mem_rep \<Rightarrow> ocaml_int"
+  ocaml_mem_rep_pbytes_mk :: "ocaml_int \<Rightarrow> ocaml_char \<Rightarrow> mem_rep"
+  ocaml_mem_rep_pbytes_byte_at :: "mem_rep \<Rightarrow> ocaml_int \<Rightarrow> ocaml_char"
+  ocaml_mem_rep_pbytes_read_bytes :: "mem_rep \<Rightarrow> ocaml_int \<Rightarrow> ocaml_int \<Rightarrow> ocaml_char list"
+  ocaml_mem_rep_pbytes_write_bytes :: "mem_rep \<Rightarrow> ocaml_int \<Rightarrow> ocaml_char list \<Rightarrow> mem_rep"
+  ocaml_mem_rep_pbytes_append :: "mem_rep \<Rightarrow> ocaml_int \<Rightarrow> ocaml_char \<Rightarrow> mem_rep"
+  ocaml_mem_rep_pbytes_set_int8 :: "mem_rep \<Rightarrow> ocaml_int \<Rightarrow> ocaml_int \<Rightarrow> mem_rep"
+  ocaml_mem_rep_pbytes_get_int8 :: "mem_rep \<Rightarrow> ocaml_int \<Rightarrow> ocaml_int"
+  ocaml_mem_rep_pbytes_set_uint8 :: "mem_rep \<Rightarrow> ocaml_int \<Rightarrow> ocaml_int \<Rightarrow> mem_rep"
+  ocaml_mem_rep_pbytes_get_uint8 :: "mem_rep \<Rightarrow> ocaml_int \<Rightarrow> ocaml_int"
+  ocaml_mem_rep_pbytes_set_int16 :: "mem_rep \<Rightarrow> ocaml_int \<Rightarrow> ocaml_int \<Rightarrow> mem_rep"
+  ocaml_mem_rep_pbytes_get_int16 :: "mem_rep \<Rightarrow> ocaml_int \<Rightarrow> ocaml_int"
+  ocaml_mem_rep_pbytes_set_uint16 :: "mem_rep \<Rightarrow> ocaml_int \<Rightarrow> ocaml_int \<Rightarrow> mem_rep"
+  ocaml_mem_rep_pbytes_get_uint16 :: "mem_rep \<Rightarrow> ocaml_int \<Rightarrow> ocaml_int"
+  ocaml_mem_rep_pbytes_set_int32 :: "mem_rep \<Rightarrow> ocaml_int \<Rightarrow> ocaml_i32 \<Rightarrow> mem_rep"
+  ocaml_mem_rep_pbytes_get_int32 :: "mem_rep \<Rightarrow> ocaml_int \<Rightarrow> ocaml_i32"
+  ocaml_mem_rep_pbytes_set_int64 :: "mem_rep \<Rightarrow> ocaml_int \<Rightarrow> ocaml_i64 \<Rightarrow> mem_rep"
+  ocaml_mem_rep_pbytes_get_int64 :: "mem_rep \<Rightarrow> ocaml_int \<Rightarrow> ocaml_i64"
 
 code_printing
-  type_constructor mem_rep \<rightharpoonup> (OCaml) "uint8 Parray.t"
-| constant ocaml_mem_rep_mk \<rightharpoonup> (OCaml) "Parray.make"
-| constant ocaml_mem_rep_length  \<rightharpoonup> (OCaml) "Parray.length"
-| constant ocaml_mem_rep_byte_at \<rightharpoonup> (OCaml) "MemRepWrapper.memRepByteAt"
-| constant ocaml_mem_rep_read_bytes \<rightharpoonup> (OCaml) "MemRepWrapper.memRepReadBytes"
-| constant ocaml_mem_rep_write_bytes \<rightharpoonup> (OCaml) "MemRepWrapper.memRepWriteBytes"
-| constant ocaml_mem_rep_append \<rightharpoonup> (OCaml) "MemRepWrapper.memRepAppend"
+  type_constructor mem_rep \<rightharpoonup> (OCaml) "Pbytes.pbt"
+| constant ocaml_mem_rep_pbytes_mk \<rightharpoonup> (OCaml) "Pbytes.make "
+| constant ocaml_mem_rep_pbytes_length  \<rightharpoonup> (OCaml) "Pbytes.length"
+| constant ocaml_mem_rep_pbytes_byte_at \<rightharpoonup> (OCaml) "MemRepWrapper.memRepByteAt"
+| constant ocaml_mem_rep_pbytes_read_bytes \<rightharpoonup> (OCaml) "MemRepWrapper.memRepReadBytes"
+| constant ocaml_mem_rep_pbytes_write_bytes \<rightharpoonup> (OCaml) "MemRepWrapper.memRepWriteBytes"
+| constant ocaml_mem_rep_pbytes_append \<rightharpoonup> (OCaml) "MemRepWrapper.memRepAppend"
+| constant ocaml_mem_rep_pbytes_set_int8 \<rightharpoonup> (OCaml) "Pbytes.set'_int8"
+| constant ocaml_mem_rep_pbytes_get_int8 \<rightharpoonup> (OCaml) "Pbytes.get'_int8"
+| constant ocaml_mem_rep_pbytes_set_uint8 \<rightharpoonup> (OCaml) "Pbytes.set'_uint8"
+| constant ocaml_mem_rep_pbytes_get_uint8 \<rightharpoonup> (OCaml) "Pbytes.get'_uint8"
+| constant ocaml_mem_rep_pbytes_set_int16 \<rightharpoonup> (OCaml) "Pbytes.set'_int16"
+| constant ocaml_mem_rep_pbytes_get_int16 \<rightharpoonup> (OCaml) "Pbytes.get'_int16"
+| constant ocaml_mem_rep_pbytes_set_uint16 \<rightharpoonup> (OCaml) "Pbytes.set'_uint16"
+| constant ocaml_mem_rep_pbytes_get_uint16 \<rightharpoonup> (OCaml) "Pbytes.get'_uint16"
+| constant ocaml_mem_rep_pbytes_set_int32 \<rightharpoonup> (OCaml) "Pbytes.set'_int32"
+| constant ocaml_mem_rep_pbytes_get_int32 \<rightharpoonup> (OCaml) "Pbytes.get'_int32"
+| constant ocaml_mem_rep_pbytes_set_int64 \<rightharpoonup> (OCaml) "Pbytes.set'_int64"
+| constant ocaml_mem_rep_pbytes_get_int64 \<rightharpoonup> (OCaml) "Pbytes.get'_int64"
 
 axiomatization where
-  mem_rep_length_is[code]: "mem_rep_length m \<equiv> ocaml_int_to_nat (ocaml_mem_rep_length m)" and
-  mem_rep_byte_at_is[code]: "mem_rep_byte_at m x \<equiv> (ocaml_mem_rep_byte_at m (nat_to_ocaml_int x))" and
-  mem_rep_read_bytes_is[code]: "mem_rep_read_bytes m x y \<equiv> ocaml_mem_rep_read_bytes m (nat_to_ocaml_int x) (nat_to_ocaml_int y)" and
-  mem_rep_write_bytes_is[code]: "mem_rep_write_bytes m x bs \<equiv> ocaml_mem_rep_write_bytes m (nat_to_ocaml_int x) bs" and
-  mem_rep_append_is[code]: "mem_rep_append m x b \<equiv> ocaml_mem_rep_append m (nat_to_ocaml_int x) b" and
-  mem_rep_mk_is[code]: "mem_rep_mk x = ocaml_mem_rep_mk (nat_to_ocaml_int (x * Ki64)) zero_byte"
+  mem_rep_length_is[code]: "mem_rep_length m \<equiv> ocaml_int_to_nat (ocaml_mem_rep_pbytes_length m)" and
+  mem_rep_byte_at_is[code]: "mem_rep_byte_at m x \<equiv> ocaml_char_to_isabelle_byte (ocaml_mem_rep_pbytes_byte_at m (nat_to_ocaml_int x))" and
+  mem_rep_read_bytes_is[code]: "mem_rep_read_bytes m x y \<equiv> map ocaml_char_to_isabelle_byte (ocaml_mem_rep_pbytes_read_bytes m (nat_to_ocaml_int x) (nat_to_ocaml_int y))" and
+  mem_rep_write_bytes_is[code]: "mem_rep_write_bytes m x bs \<equiv> ocaml_mem_rep_pbytes_write_bytes m (nat_to_ocaml_int x) (map isabelle_byte_to_ocaml_char bs)" and
+  mem_rep_append_is[code]: "mem_rep_append m x b \<equiv> ocaml_mem_rep_pbytes_append m (nat_to_ocaml_int x) (isabelle_byte_to_ocaml_char b)" and
+  mem_rep_mk_is[code]: "mem_rep_mk x = ocaml_mem_rep_pbytes_mk (nat_to_ocaml_int (x * Ki64)) (isabelle_byte_to_ocaml_char zero_byte)" and
+  
+  mem_rep_write_i32_is[code]: "mem_rep_write_i32 m n val = ocaml_mem_rep_pbytes_set_int32 m (nat_to_ocaml_int n) (isabelle_int32_to_ocaml_int32 val)" and
+  mem_rep_read_i32_is[code]: "mem_rep_read_i32 m n = ocaml_int32_to_isabelle_int32 (ocaml_mem_rep_pbytes_get_int32 m (nat_to_ocaml_int n))" and
+  mem_rep_write_i64_is[code]: "mem_rep_write_i64 m n vi64 = ocaml_mem_rep_pbytes_set_int64 m (nat_to_ocaml_int n) (isabelle_int64_to_ocaml_int64 vi64)" and
+  mem_rep_read_i64_is[code]: "mem_rep_read_i64 m n = ocaml_int64_to_isabelle_int64 (ocaml_mem_rep_pbytes_get_int64 m (nat_to_ocaml_int n))" and
+  mem_rep_write_f32_is[code]: "mem_rep_write_f32 m n vf32 = ocaml_mem_rep_pbytes_set_int32 m (nat_to_ocaml_int n) (ocaml_i32_reinterpret_f32 vf32)" and
+  mem_rep_read_f32_is[code]: "mem_rep_read_f32 m n = ocaml_f32_reinterpret_i32 (ocaml_mem_rep_pbytes_get_int32 m (nat_to_ocaml_int n))" and
+  mem_rep_write_f64_is[code]: "mem_rep_write_f64 m n vf64 = ocaml_mem_rep_pbytes_set_int64 m (nat_to_ocaml_int n) (ocaml_i64_reinterpret_f64 vf64)" and
+  mem_rep_read_f64_is[code]: "mem_rep_read_f64 m n = ocaml_f64_reinterpret_i64 (ocaml_mem_rep_pbytes_get_int64 m (nat_to_ocaml_int n))" and
+  
+  mem_rep_write_i8_of_i32_is[code]: "mem_rep_read_i32_of_i8 m n = ocaml_int32_to_isabelle_int32 (ocaml_int_to_ocaml_i32_s (ocaml_mem_rep_pbytes_get_int8 m (nat_to_ocaml_int n)))" and
+  mem_rep_write_u8_of_i32_is[code]: "mem_rep_read_i32_of_u8 m n = ocaml_int32_to_isabelle_int32 (ocaml_int_to_ocaml_i32_s (ocaml_mem_rep_pbytes_get_uint8 m (nat_to_ocaml_int n)))" and  
+  mem_rep_write_i16_of_i32_is[code]: "mem_rep_read_i32_of_i16 m n = ocaml_int32_to_isabelle_int32 (ocaml_int_to_ocaml_i32_s (ocaml_mem_rep_pbytes_get_int16 m (nat_to_ocaml_int n)))" and  
+  mem_rep_write_u16_of_i32_is[code]: "mem_rep_read_i32_of_u16 m n = ocaml_int32_to_isabelle_int32 (ocaml_int_to_ocaml_i32_s (ocaml_mem_rep_pbytes_get_uint16 m (nat_to_ocaml_int n)))" and  
+  mem_rep_write_i32_of_i32_is[code]: "mem_rep_read_i32_of_i32 m n = ocaml_int32_to_isabelle_int32 (ocaml_mem_rep_pbytes_get_int32 m (nat_to_ocaml_int n))" and  
+  mem_rep_write_u32_of_i32_is[code]: "mem_rep_read_i32_of_u32 m n = ocaml_int32_to_isabelle_int32 (ocaml_mem_rep_pbytes_get_int32 m (nat_to_ocaml_int n))" and
+  
+  mem_rep_write_i8_of_i64_is[code]: "mem_rep_read_i64_of_i8 m n = ocaml_int64_to_isabelle_int64 (ocaml_int_to_ocaml_i64_s (ocaml_mem_rep_pbytes_get_int8 m (nat_to_ocaml_int n)))" and
+  mem_rep_write_u8_of_i64_is[code]: "mem_rep_read_i64_of_u8 m n = ocaml_int64_to_isabelle_int64 (ocaml_int_to_ocaml_i64_s (ocaml_mem_rep_pbytes_get_uint8 m (nat_to_ocaml_int n)))" and  
+  mem_rep_write_i16_of_i64_is[code]: "mem_rep_read_i64_of_i16 m n = ocaml_int64_to_isabelle_int64 (ocaml_int_to_ocaml_i64_s (ocaml_mem_rep_pbytes_get_int16 m (nat_to_ocaml_int n)))" and  
+  mem_rep_write_u16_of_i64_is[code]: "mem_rep_read_i64_of_u16 m n = ocaml_int64_to_isabelle_int64 (ocaml_int_to_ocaml_i64_s (ocaml_mem_rep_pbytes_get_uint16 m (nat_to_ocaml_int n)))" and  
 
+  mem_rep_write_i32_of_i64_is[code]: "mem_rep_read_i64_of_i32 m n = wasm_extend_s (ocaml_int32_to_isabelle_int32 (ocaml_mem_rep_pbytes_get_int32 m (nat_to_ocaml_int n)))" and  
+  mem_rep_write_u32_of_i64_is[code]: "mem_rep_read_i64_of_u32 m n = wasm_extend_u (ocaml_int32_to_isabelle_int32 (ocaml_mem_rep_pbytes_get_int32 m (nat_to_ocaml_int n)))"
 end
